cleanup

LeanLambdaLibMathlib/src/term.lean
@@ -1,142 +1,846 @@
-import Qq
-import Lean
-open Lean Elab Meta Term Meta Command Qq Match PrettyPrinter Delaborator SubExpr
+-- this file is a proof of confluence of lambda-beta-eta
+-- i very roughly followed Nipkow (2001), although i did many parts differently
 
-def Ctx := List String
+import Mathlib.Tactic.ApplyFun
 
-inductive Var : Ctx → String → Type
-| zero : ∀ {Γ}, (s : String) -> Var (s :: Γ) s
-| succ : ∀ {Γ s s'}, Var Γ s' → Var (s :: Γ) s'
+inductive Constant
+| strConst : String -> Constant
 
-inductive Term : Ctx → Type
-| const : ∀ {Γ}, String → Term Γ
-| var : ∀ {Γ}, (s : String) → Var Γ s → Term Γ
-| lam : ∀ {Γ}, (s : String) → Term (s :: Γ) → Term Γ
-| app : ∀ {Γ}, Term Γ → Term Γ → Term Γ
+inductive Term : Type
+| var : Nat → Term
+| const : Constant → Term
+| lam : String -> Term → Term
+| app : Term → Term → Term
 
-declare_syntax_cat lambda_scope
-syntax ident : lambda_scope
+open Term
 
-syntax:10 (name := lambda_scoper) "<" lambda_scope:10 ">" : term
-syntax "(" lambda_scope ")" : lambda_scope
-syntax "{" term:10 "}" : lambda_scope
-syntax:60 lambda_scope:60 lambda_scope:61 : lambda_scope
-syntax "λ" ident+ ". " lambda_scope : lambda_scope
+def lift (k : Nat) (t : Term) : Term :=
+  match t with
+  -- | var i => if i >= k then Term.var (Nat.succ i) else Term.var i
+  | var i => Term.var (if i >= k then Nat.succ i else i)
+  | const c => const c
+  | lam s t => lam s (lift (Nat.succ k) t)
+  | app t1 t2 => app (lift k t1) (lift k t2)
 
-partial def buildVarFromCtx (name : String) (ctx : Q(Ctx)) : MetaM Expr := -- MetaM Q(Var ctx) :=
-  match ctx with
-  | ~q(List.cons $name2 $rest) =>
-    if name2 == Expr.lit (Literal.strVal name)
-      then return q(@Var.zero $rest $name)
-      else do let i : Q(Var $rest $name) <- buildVarFromCtx name q($rest)
-              return q(@Var.succ $rest $name2 $name $i)
-              -- return q(@Var.succ $rest $name2 $i)
-  | _ => throwError (String.join ["variable `", name, "' not found"])
+def subst (k : Nat) (toSub : Term) (t : Term) : Term :=
+  match t with
+  | var i => if k < i then Term.var (Nat.pred i) else if i == k then toSub else Term.var i
+  | const c => const c
+  | lam s t => lam s (subst (Nat.succ k) (lift 0 toSub) t)
+  | app t1 t2 => app (subst k toSub t1) (subst k toSub t2)
 
-def elabVarFromStringImpl (typ : Q(Type)) : MetaM Expr := do
-  let ~q(Var $ctx $name) := typ | throwError "bad"
-  return ctx
+inductive Step : Term → Term → Prop where
+| app1 : ∀{L L' M : Term},
+    Step L L'
+    → Step (app L M) (app L' M)
+| app2 : ∀{L M M' : Term},
+    Step M M'
+    → Step (app L M) (app L M')
+| beta : ∀ {s} {N : Term} {M : Term},
+    Step (app (lam s N) M) (subst 0 M N)
+| lam : ∀ {s} {N N' : Term},
+    Step N N' → Step (lam s N) (lam s N')
 
-syntax (name := namedvarelab) "namedvar" ident : term
+-------------------------------------------------------------------------------------
+-- everyone's favorite part of these kind of proofs : a bzillion subst/lift lemmas --
+-------------------------------------------------------------------------------------
 
-@[term_elab namedvarelab]
-def elabVarFromString : TermElab := fun stx typ? => do
-  -- TODO: try out the effect of having or not having this line
-  tryPostponeIfNoneOrMVar typ?
-  let some typ := typ? | throwError "expected type error"
-  let `(namedvar $s:ident) := stx | throwError "something"
-  let ctx <- elabVarFromStringImpl typ
-  tryPostponeIfNoneOrMVar ctx
-  buildVarFromCtx (toString s.getId) ctx
+-- my strategy picking these lemmas is: they are those necessary to bring expressions
+-- to a normal form where all lifts are inside substs, lifts are in decreasing index order,
+-- substs are in increasing index order, and also any further lemmas that ended up being necessary
 
-def firstLetterCapital (s : String) : Bool :=
-  Char.isUpper (String.front s)
+theorem lift_lift (i1 i2 : Nat) (t : Term) (H : i2 < i1) :
+    lift i1 (lift i2 t) = lift i2 (lift (Nat.pred i1) t) := by
+  revert i1 i2
+  induction t with
+  | var i =>
+    intros
+    repeat (first | simp [lift] | split | cutsat)
+  | const c =>
+    intros
+    simp [lift]
+  | lam s t ih =>
+    intros
+    simp [lift]
+    rw [ih] <;> try cutsat
+    repeat (first | simp | split | cutsat | contradiction)
+  | app t1 t2 ih1 ih2 =>
+    intros
+    simp [lift]
+    rw [ih1, ih2]
+    repeat (first | simp | split | cutsat | contradiction)
 
--- heavily referenced https://stackoverflow.com/questions/79575084/lean4-lambda-calculus-dsl-macro
-macro_rules
-  | `(< λ $xs:ident* . $body:lambda_scope >) => do
-    let mut acc <- `(< $body >)
-    for x in xs.reverse do
-      acc <- `(Term.lam $(Lean.quote (toString x.getId)) $acc)
-    return acc
-  | `(< $x:lambda_scope $xs:lambda_scope >) => do
-    `(Term.app (< $x >) (< $xs >))
-  | `(< $s:ident >) =>
-    let str := toString s.getId
-    if firstLetterCapital str
-      then `(Term.const $(Lean.quote str))
-      else `(Term.var $(Lean.quote str) (namedvar $s))
-  | `(< ($t:lambda_scope) >) => `(< $t >)
-  | `(< { $t:term } >) => `($t)
+theorem lift_subst (i1 i2 : Nat) (t1 t : Term) :
+    lift i1 (subst i2 t1 t) =
+      if i1 < i2
+        then subst (Nat.succ i2) (lift i1 t1) (lift i1 t)
+        else subst i2 (lift i1 t1) (lift (Nat.succ i1) t) := by
+  revert i1 i2 t1
+  induction t with
+  | var i =>
+    intros
+    repeat (first | simp [subst, lift] | split | cutsat | contradiction)
+  | const c =>
+    intros
+    simp [subst, lift]
+  | lam s t ih =>
+    intros
+    simp [subst, lift]
+    rw [ih]
+    simp
+    rw [lift_lift]
+    repeat (first | simp | split | cutsat | contradiction)
+  | app t1 t2 ih1 ih2 =>
+    intros
+    simp [subst, lift]
+    rw [ih1, ih2]
+    repeat (first | simp | split | cutsat | contradiction)
+
+theorem subst_lift (i : Nat) (t1 t2 : Term) : subst i t1 (lift i t2) = t2 := by
+  revert i t1
+  induction t2 with
+  | var i =>
+    intros
+    repeat (first | simp [subst, lift] | split | cutsat | contradiction)
+  | const c =>
+    intros
+    simp [subst, lift]
+  | lam s t ih =>
+    intros
+    simp [subst, lift]
+    rw [ih]
+  | app t1 t2 ih1 ih2 =>
+    intros
+    simp [subst, lift]
+    rw [ih1, ih2]
+    repeat (first | simp | split | cutsat | contradiction)
+
+theorem subst_lift_off_by_1 (i1 i2 : Nat) (t1 t : Term) (H : i1 = i2 + 1) :
+    subst i1 t1 (lift i2 t) = subst i2 t1 (lift i1 t) := by
+  revert i1 i2 H t1
+  induction t with
+  | var i =>
+    intros
+    repeat (first | simp [subst, lift] | split | cutsat | contradiction)
+  | const c =>
+    intros
+    simp [subst, lift]
+  | lam s t ih =>
+    intros
+    simp [subst, lift]
+    rw [ih]
+    cutsat
+  | app t1 t2 ih1 ih2 =>
+    intros
+    simp [subst, lift]
+    rw [ih1, ih2]
+    repeat (first | simp | split | cutsat | contradiction)
 
 
-@[app_unexpander Term.const]
-def unexpandConst : Unexpander
-  | `($_const $x:str) =>
-    let str := x.getString
-    let name : Syntax := mkIdent $ Name.mkSimple str
-    let tname : TSyntax _ := {raw := name}
-    `(< $tname >)
-  | _ => throw ()
+theorem subst_subst (i1 i2 : Nat) (t1 t2 t : Term) (H : i1 >= i2) :
+    subst i1 t1 (subst i2 t2 t) =
+      subst i2 (subst i1 t1 t2) (subst (Nat.succ i1) (lift i2 t1) t) := by
+  revert i1 i2 t1 t2
+  induction t with
+  | var i =>
+    intros
+    repeat' (first | simp [subst] | split | cutsat | contradiction | rw [subst_lift])
+  | const c =>
+    intros
+    simp [subst]
+  | lam s t ih =>
+    intros
+    simp [subst]
+    rw [ih] <;> try cutsat
+    simp
+    rw [lift_lift] <;> try cutsat
+    rw [lift_subst]
+    repeat' (first | simp | split | cutsat )
+    rewrite [subst_lift_off_by_1] <;> cutsat
+  | app t1 t2 ih1 ih2 =>
+    intros
+    simp [subst]
+    rw [ih1, ih2]
+    repeat (first | simp | split | cutsat | contradiction)
 
-@[app_unexpander Term.lam]
-def unexpandLam : Unexpander
-  | `($_  $name:str $body) =>
-    let ident := mkIdent $ Name.mkSimple name.getString
-    match body with
-    | `(< λ $idents:ident* . $body2 >) => `(< λ $ident $idents* . $body2 >) -- this case handles nested lambdas
-    | `(< $inside >) => `(< λ $ident . $inside >)
-    | `( $inside ) => `(< λ $ident . {$inside} >)
-    -- | _ => throw ()
-  | _ => throw ()
+theorem lift_injective {i : Nat} {M N : Term} (H : lift i M = lift i N) : M = N := by
+  revert i N H
+  induction M with
+  | var i =>
+    intros i N H
+    cases N <;> try contradiction
+    simp [lift] at H
+    repeat' (first | split at H | cutsat)
+  | const c =>
+    intros i N H
+    cases N <;> try contradiction
+    simp [lift] at H
+    subst c
+    rfl
+  | lam s t ih =>
+    intros i N H
+    cases N <;> try contradiction
+    simp [lift] at H
+    cases H with | intro H1 H2
+    subst s
+    rw [ih H2]
+  | app t1 t2 ih1 ih2 =>
+    intros i N H
+    cases N <;> try contradiction
+    simp [lift] at H
+    cases H with | intro H1 H2
+    rw [ih1 H1]
+    rw [ih2 H2]
 
-inductive ParenKind where
-| None
-| Parens
-| Braces
+theorem subst_lift_2 (i : Nat) {t : Term} :
+    t = subst i (var i) (lift (Nat.succ i) t) := by
+  revert i
+  induction t with
+  | var i =>
+    intros i
+    simp [subst, lift]
+    repeat' (first | split | cutsat )
+  | const c =>
+    intros i
+    rfl
+  | lam s t ih =>
+    intros i
+    simp [lift, subst]
+    apply ih (Nat.succ i)
+  | app t1 t2 ih1 ih2 =>
+    intros i
+    simp [subst, lift]
+    apply And.intro
+    · apply ih1
+    · apply ih2
 
-open ParenKind
+--------------------------------------------------------------------------------
+---------- A proof of confluence for beta alone without eta -------------------
+--------------------------------------------------------------------------------
 
-@[app_unexpander Term.app]
-def unexpandApp : Unexpander
-  -- | `($_ (< $a:lambda_scope > : term) (< $b:lambda_scope > : term)) =>
-  | `($_ $a_term $b_term) =>
-    let a_in := match a_term with
-      | `(< $a >) => a
-      | _ => TSyntax.mk Syntax.missing
-    let b_in := match b_term with
-      | `(< $b >) => b
-      | _ => TSyntax.mk Syntax.missing
-        -- we need to decide when to add parentheses.
-        -- if a is lambda parenth it, if b is app or lambda parenth it
-    let parena := match a_term with
-      | `(< λ $_xs:ident* . $_body:lambda_scope >) => Parens
-      | `(< $_any >) => None
-      | _ => Braces
-    let parenb := match b_term with
-      | `(< λ $_xs:ident* . $_body:lambda_scope >) => Parens
-      | `(< $_x:lambda_scope $_xs:lambda_scope >) => Parens
-      | `(< $_any >) => None
-      | _ => Braces
-    -- because we can only match on things and construct syntax in the term category and not
-    -- the lambda_scope category, there is no way to avoid this code repetition.
-    match parena, parenb with
-    | Parens, Parens => `(< ($a_in) ($b_in) >)
-    | Parens, None => `(< ($a_in) $b_in >)
-    | None, Parens => `(< $a_in ($b_in) >)
-    | None, None => `(< $a_in $b_in >)
-    | Braces, Braces => `(< {$a_term} {$b_term} >)
-    | Braces, Parens => `(< {$a_term} ($b_in) >)
-    | Braces, None => `(< {$a_term} $b_in >)
-    | Parens, Braces => `(< ($a_in) {$b_term} >)
-    | None, Braces => `(< $a_in {$b_term} >)
-  | _ => throw ()
+inductive Par : Term → Term → Prop
+| pvar : ∀{x : Nat}, Par (var x) (var x)
+| pconst : ∀{c : Constant}, Par (const c) (const c)
+| plam : ∀{s} {N N' : Term},
+  Par N N' → Par (lam s N) (lam s N')
+| papp : ∀{L L' M M' : Term},
+  Par L L' → Par M M' → Par (app L M) (app L' M')
+| pbeta : ∀{s} {N N' : Term} {M M' : Term},
+  Par N N' → Par M M' → Par (app (lam s N) M) (subst 0 M' N')
 
-@[app_unexpander Term.var]
-def unexpandVar : Unexpander
-  | `($_var $x:str $_dontcare) =>
-    let str:= x.getString
-    let name : Syntax := mkIdent $ Name.mkSimple str
-    let tname : TSyntax _ := {raw := name}
-    `(< $tname >)
-  | _ => throw ()
+theorem parRefl {t : Term} : Par t t := by
+  induction t <;> constructor <;> repeat assumption
+
+theorem parLift {i} {M M' : Term}
+  (p : Par M M')
+  : Par (lift i M) (lift i M') := by
+  revert i
+  induction p with
+  | @pvar x => intros; simp [lift]; split<;> apply Par.pvar
+  | pconst => intros; constructor
+  | plam _p ih => intros; simp [lift]; apply Par.plam; apply ih
+  | papp _p1 _p2 ih1 ih2 => intros; simp [lift]; apply (Par.papp ih1 ih2)
+  | pbeta _p1 _p2 ih1 ih2 =>
+    intros
+    simp [lift]
+    rw [lift_subst]
+    apply Par.pbeta
+    · apply ih1
+    · apply ih2
+
+theorem parSubst {i} {N N'} {M M' : Term}
+  (p1 : Par N N')
+  (p2 : Par M M')
+  : Par (subst i N M) (subst i N' M') := by
+  revert i N N'
+  induction p2 with
+  | @pvar x =>
+    intros; simp [subst]; split
+    · apply parRefl
+    · split
+      · assumption
+      · apply parRefl
+  | pconst => intros; constructor
+  | plam _p ih =>
+    intros i N N' pNN'
+    simp [subst]; apply Par.plam; apply ih
+    apply parLift
+    apply pNN'
+  | papp _p1 _p2 ih1 ih2 =>
+    intros i N N' pNN'
+    simp [subst]; apply (Par.papp (ih1 pNN') (ih2 pNN'))
+  | @pbeta s a a' b b' _p1 _p2 ih1 ih2 =>
+    intros i N N' pNN'
+    rw [subst_subst] <;> try cutsat
+    simp [subst]
+    apply Par.pbeta
+    · apply (ih1 (parLift pNN'))
+    · apply (ih2 pNN')
+
+theorem parDiamond {t t1 t2 : Term}
+  (p1 : Par t t1) (p2 : Par t t2)
+  : ∃ t', Par t1 t' ∧ Par t2 t' :=
+  match p1, p2 with
+  | Par.pvar, Par.pvar => ⟨_, Par.pvar, Par.pvar⟩
+  | Par.pconst, Par.pconst => ⟨_, Par.pconst, Par.pconst⟩
+  | Par.papp a1 b1, Par.papp a2 b2 =>
+    let ⟨a, pa1, pa2⟩ := parDiamond a1 a2
+    let ⟨b, pb1, pb2⟩ := parDiamond b1 b2
+    ⟨app a b, Par.papp pa1 pb1, Par.papp pa2 pb2⟩
+  | Par.pbeta a1 b1, Par.pbeta a2 b2 =>
+    let ⟨a, pa1, pa2⟩ := parDiamond a1 a2
+    let ⟨b, pb1, pb2⟩ := parDiamond b1 b2
+    ⟨subst 0 b a, parSubst pb1 pa1, parSubst pb2 pa2⟩
+    -- ⟨subst 0 b a, _, _⟩
+  | Par.papp (Par.plam a1) b1, Par.pbeta a2 b2 =>
+    let ⟨a, pa1, pa2⟩ := parDiamond a1 a2
+    let ⟨b, pb1, pb2⟩ := parDiamond b1 b2
+    ⟨subst 0 b a, Par.pbeta pa1 pb1, parSubst pb2 pa2⟩
+  | Par.pbeta a1 b1, Par.papp (Par.plam a2) b2 => -- REPEATED CASE
+    let ⟨a, pa1, pa2⟩ := parDiamond a1 a2
+    let ⟨b, pb1, pb2⟩ := parDiamond b1 b2
+    ⟨subst 0 b a, parSubst pb1 pa1, Par.pbeta pa2 pb2⟩
+  | Par.plam a1, Par.plam a2 =>
+    let ⟨a, pa1, pa2⟩ := parDiamond a1 a2
+    ⟨lam _ a, Par.plam pa1, Par.plam pa2⟩
+
+--------------------------------------------------------------------------------
+------- some general facts about relations - from Nipkow (2001) ----------------
+--------------------------------------------------------------------------------
+def Relation (A : Type) : Type := A → A → Prop
+
+inductive Proof (P : Prop) : Type
+| proof : P → Proof P
+
+def closeRef {A} (R : Relation A) : Relation A :=
+  fun x y => x = y ∨ R x y
+
+def liftRef {A} {B} {R : Relation A} {R' : Relation B} {x y : A} (f : A → B)
+  (ctr : ∀ {x y}, R x y → R' (f x) (f y))
+  : closeRef R x y → closeRef R' (f x) (f y) :=
+  fun s => match s with
+  | Or.inl rfl => Or.inl rfl
+  | Or.inr s' => Or.inr (ctr s')
+
+-- transitive relflexive closure of a relation
+inductive closure {A} (R : Relation A) : A → A → Prop
+| refl : ∀{a : A}, closure R a a
+| cons : ∀{x y : A}, R x y → closure R y z  → closure R x z
+
+def oneStep {A} {R : Relation A} {x y : A} (step : R x y)
+  : closure R x y := closure.cons step closure.refl
+
+def transitivity {A} {R : Relation A} {x y z : A}
+  (step1 : closure R x y) (step2 : closure R y z)
+  : closure R x z :=
+  match step1 with
+  | closure.refl => step2
+  | closure.cons s ss => closure.cons s (transitivity ss step2)
+
+def liftCsr {A} {B} {R : Relation A} {R' : Relation B} {x y : A} (f : A → B)
+  (ctr : ∀ {x y}, R x y → R' (f x) (f y))
+  : closure R x y → closure R' (f x) (f y) :=
+  fun s => match s with
+  | closure.refl => closure.refl
+  | closure.cons xy yz => closure.cons (ctr xy) (liftCsr f ctr yz)
+
+inductive union {A} (R S : Relation A) : A → A → Prop
+| r : ∀{x y}, R x y → union R S x y
+| s : ∀{x y}, S x y → union R S x y
+
+def liftUnion {A} {B} {R S : Relation A} {R' S' : Relation B} {x y : A} (f : A → B)
+  (ctr1 : ∀ {x y}, R x y → R' (f x) (f y))
+  (ctr2 : ∀ {x y}, S x y → S' (f x) (f y))
+  : union R S x y → union R' S' (f x) (f y) :=
+  fun s => match s with
+  | union.r r => union.r (ctr1 r)
+  | union.s s => union.s (ctr2 s)
+
+def leftClosureUnion {A x y} {R S : Relation A}
+  (r : closure R x y) : closure (union R S) x y :=
+  match r with
+  | closure.refl => closure.refl
+  | closure.cons s ss => closure.cons (union.r s) (leftClosureUnion ss)
+
+def rightClosureUnion {A x y} {R S : Relation A}
+  (s : closure S x y) : closure (union R S) x y :=
+  match s with
+  | closure.refl => closure.refl
+  | closure.cons s ss => closure.cons (union.s s) (rightClosureUnion ss)
+
+def oneUnionStep {A x y} {R S : Relation A}
+  (s : union R S x y) : union (closure R) (closure S) x y :=
+  match s with
+  | union.r r => union.r (oneStep r)
+  | union.s s => union.s (oneStep s)
+
+def unionClosureToClosureUnion {A x y} {R S : Relation A}
+  (s : union (closure R) (closure S) x y) : closure (union R S) x y :=
+  match s with
+  | union.r r => leftClosureUnion r
+  | union.s s => rightClosureUnion s
+
+-- All from Nipkow paper
+def square {A} (R S T U : Relation A) : Prop :=
+  {x y z : A} → R x y → S x z → ∃ u, T y u ∧ U z u
+
+def commute {A} (R S : Relation A) : Prop := square R S S R
+def diamond {A} (R : Relation A) : Prop := commute R R
+def confluent {A} (R : Relation A) : Prop := diamond (closure R)
+
+--     x --R-- y
+--     |       |
+--     S       T
+--     |       |
+--     z --U-- u
+
+theorem stripLemma {A} {R S : Relation A}
+  (sq : square R S (closure S) (closeRef R))
+  : square R (closure S) (closure S) (closure R) :=
+  fun {_x} {y} {z} Rxy Sxz =>
+  match Sxz with
+  | closure.refl => ⟨y, closure.refl, oneStep Rxy⟩
+  | closure.cons xx' x'z =>
+    let ⟨out, s, r⟩ := sq Rxy xx'
+    match r with
+    | Or.inl p =>
+      ⟨z, transitivity s (by rw [<- p]; exact x'z), closure.refl⟩
+    | Or.inr r' =>
+      let ⟨out2, s2, r2⟩ := stripLemma sq r' x'z
+      ⟨out2, transitivity s s2, r2⟩
+
+theorem commutationLemma {A} {R S : Relation A}
+  (sq : square R S (closure S) (closeRef R))
+  : square (closure R) (closure S) (closure S) (closure R) :=
+  fun {_x} {y} {z} Rxy Sxz =>
+  match Rxy with
+  | closure.refl => ⟨z, Sxz, closure.refl⟩
+  | closure.cons xx' x'z =>
+    let ⟨_out, s, r⟩ := stripLemma sq xx' Sxz
+    let ⟨out2, s2, r2⟩ := commutationLemma sq x'z s
+    ⟨out2, s2, transitivity r r2⟩
+
+theorem commutativeUnion {A} {R S : Relation A}
+  (rConfluent : confluent R) (sConfluent : confluent S)
+  (commutes : commute (closure R) (closure S)) : confluent (union R S) :=
+  fun {x} {y} {z} =>
+  let rec commutativeUnionLemma
+    : square (union (closure R) (closure S)) (closure (union R S))
+      (closure (union R S)) (union (closure R) (closure S)) :=
+    fun {x} {y} {z} top left =>
+      match left with
+      | closure.refl => ⟨y, closure.refl, top⟩
+      | closure.cons s ss =>
+        match s, top with
+        | union.r left', union.r top' =>
+          let ⟨w', right', top''⟩ := rConfluent top' (oneStep left')
+          let ⟨w, right, bottom⟩ := commutativeUnionLemma (union.r top'') ss
+          ⟨w, transitivity (leftClosureUnion right') right, bottom⟩
+        | union.r left', union.s top' =>
+          let ⟨w', top'', right'⟩ := commutes (oneStep left') top'
+          let ⟨w, right, bottom⟩ := commutativeUnionLemma (union.s top'') ss
+          ⟨w, transitivity (leftClosureUnion right') right, bottom⟩
+        | union.s left', union.r top' =>
+          let ⟨w', right', top''⟩ := commutes top' (oneStep left')
+          let ⟨w, right, bottom⟩ := commutativeUnionLemma (union.r top'') ss
+          ⟨w, transitivity (rightClosureUnion right') right, bottom⟩
+        | union.s left', union.s top' =>
+          let ⟨w', right', top''⟩ := sConfluent top' (oneStep left')
+          let ⟨w, right, bottom⟩ := commutativeUnionLemma (union.s top'') ss
+          ⟨w, transitivity (rightClosureUnion right') right, bottom⟩
+    by
+      intro top
+      revert z
+      induction top with
+      | refl => intro z left; exact ⟨_, left, closure.refl⟩
+      | cons s _ss ih =>
+        intro z left
+        let ⟨_, right', bottom'⟩ := commutativeUnionLemma (oneUnionStep s) left
+        let ⟨out2, right, bottom⟩ := ih right'
+        exact ⟨out2, right, transitivity (unionClosureToClosureUnion bottom') bottom⟩
+
+---------------------------------------------------------------------------------
+------- Eta ---------------------------------------------------------------------
+---------------------------------------------------------------------------------
+
+def dummy : Term := const (Constant.strConst "dummy")
+
+inductive StepEta : Term → Term → Prop where
+| app1 : ∀ {L L' M : Term},
+    StepEta L L'
+    → StepEta (app L M) (app L' M)
+| app2 : ∀ {L M M' : Term},
+    StepEta M M'
+    → StepEta (app L M) (app L M')
+| lam : ∀ {s} {N N' : Term},
+    StepEta N N' → StepEta (lam s N) (lam s N')
+| eta : ∀{s} {M M' : Term},
+  M = lift 0 M'
+  → StepEta (lam s (app M (var 0))) M'
+| alpha : ∀{s1 s2} {M : Term},
+  StepEta (lam s1 M) (lam s2 M)
+
+
+theorem etaLift {i} {M M' : Term}
+  (p : StepEta M M')
+  : StepEta (lift i M) (lift i M') := by
+  revert i
+  induction p with
+  | lam _p ih => intros; simp [lift]; apply StepEta.lam; apply ih
+  | app1 _p ih => intros; simp [lift]; apply (StepEta.app1 ih)
+  | app2 _p ih => intros; simp [lift]; apply (StepEta.app2 ih)
+  | @eta s M M' p =>
+    intros
+    subst M
+    simp [lift]
+    rw [lift_lift] <;> try cutsat
+    apply StepEta.eta
+    rfl
+  | alpha =>
+    intros
+    apply StepEta.alpha
+
+theorem etaSubst1 {i} {N N'} {M : Term}
+  (p : StepEta N N')
+  : closure StepEta (subst i N M) (subst i N' M) := by
+  revert i N N' p
+  induction M with
+  | var i =>
+    intros
+    simp [subst]
+    repeat' (first | simp [subst] | split | cutsat | apply closure.refl)
+    apply oneStep
+    assumption
+  | const c =>
+    intros
+    apply closure.refl
+  | lam s t ih =>
+    intros
+    simp [subst]
+    apply (liftCsr (lam _) StepEta.lam)
+    apply ih
+    apply etaLift
+    assumption
+  | app t1 t2 ih1 ih2 =>
+    intros
+    apply transitivity
+    · apply (liftCsr (fun x => app x _) StepEta.app1)
+      apply ih1
+      assumption
+    · apply (liftCsr (app _) StepEta.app2)
+      apply ih2
+      assumption
+
+theorem etaSubst2 (i N) {M M' : Term}
+  (p : StepEta M M')
+  : StepEta (subst i N M) (subst i N M') := by
+  revert i N
+  induction p with
+  | lam _p ih =>
+    intros
+    simp [subst]
+    --
+    apply StepEta.lam
+    apply ih
+  | app1 _p1 ih =>
+    intros
+    simp [subst]
+    apply StepEta.app1
+    apply ih
+  | app2 _p1 ih =>
+    intros
+    simp [subst]
+    apply StepEta.app2
+    apply ih
+  | alpha =>
+    intros
+    apply StepEta.alpha
+  | @eta s M M' p =>
+    intros i N
+    subst M
+    simp [subst]
+    have iamwritingaproof : subst (i + 1) (lift 0 N) (lift 0 M') = lift 0 (subst i N M') := by
+      rewrite [lift_subst]
+      split <;> try cutsat
+      rewrite [subst_lift_off_by_1] <;> try cutsat
+    rewrite [iamwritingaproof]
+    apply StepEta.eta
+    rfl
+
+theorem stepEtaRespectsLift {i : Nat} {M N : Term}
+  (step : StepEta (lift i M) N)
+  : exists N', N = lift i N' := by
+  generalize H : lift i M = x at *
+  revert i M
+  induction step with
+  | lam _p ih =>
+    intros i M H
+    cases M with | lam s t => _ | _ <;> simp [lift] at H
+    rcases H with ⟨rfl, rfl⟩
+    specialize (ih rfl)
+    rcases ih with ⟨N', rfl⟩
+    exists (lam s N')
+  | @app1 L L' R _p1 ih =>
+    intros i M H
+    cases M <;> simp [lift] at H
+    rcases H with ⟨rfl, rfl⟩
+    specialize (ih rfl)
+    rcases ih with ⟨N', rfl⟩
+    exact ⟨app _ _, rfl⟩
+  | app2 _p1 ih =>
+    intros i M H
+    cases M <;> simp [lift] at H
+    rcases H with ⟨rfl, rfl⟩
+    specialize (ih rfl)
+    rcases ih with ⟨N', rfl⟩
+    exact ⟨app _ _, rfl⟩
+  | alpha =>
+    intros i M H
+    cases M with | lam s t => _ | _ <;> simp [lift] at H
+    rcases H with ⟨rfl, rfl⟩
+    exact ⟨lam _ t, rfl⟩
+  | @eta s M M' p =>
+    intros i M' H
+    subst M
+    cases M' with | lam s t => _ | _  <;> simp [lift] at H
+    rcases H with ⟨rfl, H⟩
+    cases t with | app l r => _ | _  <;> simp [lift] at H
+    rcases H with ⟨q, H⟩
+    clear H
+    apply_fun (subst 0 (lift i dummy)) at q
+    rewrite [subst_lift] at q
+    have coolfact : subst 0 (lift i dummy) (lift (i + 1) l) = lift i (subst 0 dummy l) := by
+      rw [lift_subst]
+      simp -- TODO: how does simp solve this goal?
+    rewrite [coolfact] at q
+    exists (subst 0 dummy l)
+    subst M'
+    rfl
+
+theorem substStep (i N) {M M' : Term}
+  (step : Step M M')
+  : Step (subst i N M) (subst i N M') :=
+  match step with
+  | Step.app1 p => Step.app1 (substStep i N p)
+  | Step.app2 p => Step.app2 (substStep i N p)
+  | Step.lam p => Step.lam (substStep _ _ p)
+  | Step.beta => by
+    simp [subst]
+    rw [subst_subst] <;> try cutsat
+    apply Step.beta
+
+theorem stepRespectsLift {i : Nat} {M N : Term}
+  (step : Step (lift i M) N)
+  : exists N', N = lift i N' := by
+  generalize H : lift i M = x at *
+  revert i M
+  induction step with
+  | lam _p ih =>
+    intros i M H
+    cases M with | lam s t => _ | _ <;> simp [lift] at H
+    rcases H with ⟨rfl, rfl⟩
+    specialize (ih rfl)
+    rcases ih with ⟨N', rfl⟩
+    exists (lam s N')
+  | @app1 L L' R _p1 ih =>
+    intros i M H
+    cases M <;> simp [lift] at H
+    rcases H with ⟨rfl, rfl⟩
+    specialize (ih rfl)
+    rcases ih with ⟨N', rfl⟩
+    exact ⟨app _ _, rfl⟩
+  | app2 _p1 ih =>
+    intros i M H
+    cases M <;> simp [lift] at H
+    rcases H with ⟨rfl, rfl⟩
+    specialize (ih rfl)
+    rcases ih with ⟨N', rfl⟩
+    exact ⟨app _ _, rfl⟩
+  | beta =>
+    intros i M H
+    cases M with simp [lift] at H | app l r => _
+    rcases H with ⟨H, rfl⟩
+    cases l with simp [lift] at H | lam s t => _
+    rcases H with ⟨rfl, rfl⟩
+    exists (subst 0 r t)
+    rw [lift_subst]
+    split; try cutsat
+    rfl
+
+theorem etaProperty : square StepEta StepEta
+  (closeRef StepEta) (closeRef StepEta) :=
+  fun p1 p2 =>
+  match p1, p2 with
+  | StepEta.app1 s1, StepEta.app1 s2 =>
+    let ⟨u, bla1, bla2⟩ := etaProperty s1 s2
+    ⟨app u _, liftRef (fun x => app x _) StepEta.app1 bla1,
+      liftRef (fun x => app x _) StepEta.app1 bla2⟩
+  | StepEta.app1 s1, StepEta.app2 s2 =>
+    ⟨_, Or.inr (StepEta.app2 s2), Or.inr (StepEta.app1 s1)⟩
+  | StepEta.app2 s1, StepEta.app1 s2 => -- REPEATED CASE
+    ⟨_, Or.inr (StepEta.app1 s2), Or.inr (StepEta.app2 s1)⟩
+  | StepEta.app2 s1, StepEta.app2 s2 =>
+    let ⟨u, bla1, bla2⟩ := etaProperty s1 s2
+    ⟨app _ u, liftRef (app _) StepEta.app2 bla1, liftRef (app _) StepEta.app2 bla2⟩
+  | StepEta.lam s1, StepEta.lam s2 =>
+    let ⟨u, bla1, bla2⟩ := etaProperty s1 s2
+    ⟨lam _ u, liftRef (lam _) StepEta.lam bla1, liftRef (lam _) StepEta.lam bla2⟩
+  | StepEta.eta p, StepEta.eta p' =>
+    ⟨_, Or.inl rfl, Or.inl (lift_injective (Eq.trans (Eq.symm p') p)) ⟩
+  | StepEta.lam (StepEta.app1 s), StepEta.eta p => by
+    subst_vars
+    have s' := etaSubst2 0 dummy s
+    have ⟨N', p⟩ := stepEtaRespectsLift s
+    subst_vars
+    rw [subst_lift] at s'
+    refine ⟨_, Or.inr (StepEta.eta ?_), Or.inr s'⟩
+    rw [subst_lift]
+  | StepEta.eta p, StepEta.lam (StepEta.app1 s) => by -- REPEATED CASE
+    subst_vars
+    have s' := etaSubst2 0 dummy s
+    have ⟨N', p⟩ := stepEtaRespectsLift s
+    subst_vars
+    rw [subst_lift] at s'
+    refine ⟨_, Or.inr s', Or.inr (StepEta.eta ?_)⟩
+    rw [subst_lift]
+  | @StepEta.alpha _ s M, StepEta.alpha => ⟨lam s M, Or.inr StepEta.alpha, Or.inr StepEta.alpha⟩
+  | StepEta.alpha, StepEta.lam s => ⟨_, Or.inr (StepEta.lam s), Or.inr StepEta.alpha⟩
+  | StepEta.lam s, StepEta.alpha => ⟨_, Or.inr StepEta.alpha, Or.inr (StepEta.lam s)⟩
+  | StepEta.alpha, StepEta.eta p =>
+    ⟨_, Or.inr (StepEta.eta p), Or.inl rfl⟩
+  | StepEta.eta p, StepEta.alpha => -- REPEATED CASE
+    ⟨_, Or.inl rfl, Or.inr (StepEta.eta p)⟩
+
+theorem betaEtaCommuteProperty
+  : square Step StepEta (closure StepEta) (closeRef Step) :=
+    fun {t} {tLeft} {tRight} p1 p2 =>
+    match p1, p2 with
+    | Step.app1 p1, StepEta.app1 p2 =>
+      let ⟨t', q1, q2⟩ := betaEtaCommuteProperty p1 p2
+      ⟨_, liftCsr (fun x => app x _) StepEta.app1 q1,
+        liftRef (fun x => app x _) Step.app1 q2⟩
+    | Step.app2 p1, StepEta.app2 p2 =>
+      let ⟨t', q1, q2⟩ := betaEtaCommuteProperty p1 p2
+      ⟨_, liftCsr (app _) StepEta.app2 q1,
+        liftRef (app _) Step.app2 q2⟩
+    | Step.lam p1, StepEta.lam p2 =>
+      let ⟨t', q1, q2⟩ := betaEtaCommuteProperty p1 p2
+      ⟨_, liftCsr (lam _) StepEta.lam q1,
+        liftRef (lam _) Step.lam q2⟩
+    | Step.app1 p1, StepEta.app2 p2 =>
+      ⟨_, oneStep (StepEta.app2 p2),
+        Or.inr (Step.app1 p1)⟩
+    | Step.app2 p1, StepEta.app1 p2 => -- REPEATED CASE
+      ⟨_, oneStep (StepEta.app1 p2)
+          , Or.inr (Step.app2 p1)⟩
+    | Step.beta, StepEta.app2 p => ⟨_, etaSubst1 p, Or.inr Step.beta⟩
+    | Step.beta, StepEta.app1 (StepEta.lam p) =>
+      -- ⟨_, subEta (oneStep p) closure.refl, Or.inr Step.beta⟩
+      ⟨_, oneStep (etaSubst2 _ _ p), Or.inr Step.beta⟩
+    | Step.beta, StepEta.app1 (StepEta.eta zf) => ⟨_, closure.refl, (by
+        subst_vars
+        simp [subst]
+        rw [subst_lift]
+        apply Or.inl rfl
+        )⟩
+    | Step.lam (Step.app1 s), StepEta.eta zf => by
+      subst_vars
+      have s' := substStep 0 dummy s
+      have ⟨N', p⟩ := stepRespectsLift s
+      subst_vars
+      rw [subst_lift] at s'
+      refine ⟨_, oneStep (StepEta.eta ?_), Or.inr s'⟩
+      rw [subst_lift]
+    | Step.lam Step.beta, @StepEta.eta _ _ (lam s a) zf =>
+      ⟨_,
+        oneStep (@StepEta.alpha _ s _),
+        Or.inl (by
+        --
+        simp [lift] at zf
+        rcases zf with ⟨rfl, rfl⟩
+        simp
+        apply subst_lift_2
+        )⟩
+    | Step.beta, StepEta.app1 StepEta.alpha => ⟨_, closure.refl, Or.inr (Step.beta)⟩
+    | Step.lam s, StepEta.alpha => ⟨_, oneStep StepEta.alpha, Or.inr (Step.lam s)⟩
+
+--------------------------------------------------------------------------------
+---------- Equivalence between Par and Step ------------------------------------
+--------------------------------------------------------------------------------
+
+theorem stepToPar {t1 t2 : Term}
+  (step : Step t1 t2) : Par t1 t2 :=
+  match step with
+  | Step.app1 s => Par.papp (stepToPar s) parRefl
+  | Step.app2 s => Par.papp parRefl (stepToPar s)
+  | Step.lam s => Par.plam (stepToPar s)
+  | Step.beta => Par.pbeta parRefl parRefl
+
+theorem parToMultiStep {t1 t2 : Term}
+  (par : Par t1 t2) : closure Step t1 t2 :=
+  match par with
+  | Par.pvar => closure.refl
+  | Par.pconst => closure.refl
+  | Par.papp p1 p2 => transitivity (liftCsr (fun x => app x _) Step.app1 (parToMultiStep p1))
+    (liftCsr (app _) Step.app2 (parToMultiStep p2))
+  | Par.plam s => liftCsr (lam _) Step.lam (parToMultiStep s)
+  | Par.pbeta s1 s2 => -- Can I do this case without proving substitution properties of MultiStep?
+    transitivity (transitivity
+      (liftCsr (fun x => app (lam _ x) _) (Step.app1 ∘ Step.lam) (parToMultiStep s1))
+      (liftCsr (app _) Step.app2 (parToMultiStep s2)))
+      (oneStep Step.beta)
+
+theorem multiParToMultiStep {t1 t2 : Term}
+  (par : closure Par t1 t2) : closure Step t1 t2 :=
+  match par with
+  | closure.refl => closure.refl
+  | closure.cons s ss => transitivity (parToMultiStep s) (multiParToMultiStep ss)
+
+theorem multiStepToMultiPar {t1 t2 : Term}
+  (par : closure Step t1 t2) : closure Par t1 t2 :=
+  match par with
+  | closure.refl => closure.refl
+  | closure.cons s ss => closure.cons (stepToPar s) (multiStepToMultiPar ss)
+
+--------------------------------------------------------------------------------
+---------- Collecting all of the theorems together into confluence -------------
+--------------------------------------------------------------------------------
+
+theorem diamondToProperty {A} {R : Relation A}
+  (d : diamond R)
+  : square R R (closure R) (closeRef R) :=
+  fun s1 s2 =>
+    let ⟨_, s2', s1'⟩ := d s1 s2
+    ⟨_, oneStep s2', Or.inr s1'⟩
+theorem parConfluent : confluent Par :=
+  commutationLemma (diamondToProperty parDiamond)
+theorem stepConfluent : confluent Step :=
+  fun s1 s2 =>
+    let ⟨_, s2', s1'⟩ := parConfluent (multiStepToMultiPar s1) (multiStepToMultiPar s2)
+    ⟨_, multiParToMultiStep s2', multiParToMultiStep s1'⟩
+
+theorem closeRefToClosure {A} {R : Relation A}
+  {x y}
+  (r : closeRef R x y) : closure R x y :=
+  match r with
+  | Or.inl rfl => closure.refl
+  | Or.inr r => oneStep r
+
+theorem propertyToProperty {A} {R : Relation A}
+  (sq : square R R (closeRef R) (closeRef R))
+  : square R R (closure R) (closeRef R) :=
+  fun s1 s2 =>
+    let ⟨_, s2', s1'⟩ := sq s1 s2
+    ⟨_, closeRefToClosure s2', s1'⟩
+
+theorem etaConfluent : confluent StepEta :=
+  commutationLemma (propertyToProperty etaProperty)
+
+def AllStep : Relation Term := closure (union Step StepEta)
+
+theorem confluence : confluent (union Step StepEta) :=
+  commutativeUnion stepConfluent etaConfluent (commutationLemma betaEtaCommuteProperty)
+
+---------------- definitions to be used in the quotient --------------
+
+def equiv (t1 t2 : Term) := ∃ t, AllStep t1 t /\ AllStep t2 t
